\documentclass{article}
\usepackage{amsmath}
\usepackage{amssymb}
\usepackage{textcomp}
\usepackage{gensymb}
\begin{document}

\textbf{1.3.5} Calculate the closed-surface integral $\oint \mathbf{A} \bullet \mathbf{ds}$ if $\mathbf{A =
		x\mathbf{u_x} + y\mathbf{u_y}}$ and the surface is that of a cube. Apply the divergence theorem to solve the same
integral.\@ \textit{Note: Diagram not shown.}

\vspace{24pt}

The cube has side length $2$, and one of its corners is at the origin.

\begin{equation*}
	\begin{split}
		\oint \mathbf{A} \bullet \mathbf{ds} & = \int_{y=0}^2 \int_{x=0}^2 (x\mathbf{u_x} + y\mathbf{u_y}) \bullet (\text{d}x\text{d}y\mathbf{u_x}) \\
		& \quad + \int_{y=0}^2 \int_{x=0}^2 (x\mathbf{u_x} + y\mathbf{u_y}) \bullet (\text{d}x\text{d}y(-\mathbf{u_x})) \\
		& \quad + \int_{z=0}^2 \int_{x=0}^2 (x\mathbf{u_x} + y\mathbf{u_y}) \bullet (\text{d}x\text{d}z\mathbf{u_y}) \\
		& \quad + \int_{z=0}^2 \int_{x=0}^2 (x\mathbf{u_x} + y\mathbf{u_y}) \bullet (\text{d}x\text{d}z(-\mathbf{u_y})) \\
		& \quad + \int_{z=0}^2 \int_{y=0}^2 (x\mathbf{u_x} + y\mathbf{u_y}) \bullet (\text{d}y\text{d}z\mathbf{u_y}) \\
		& \quad + \int_{z=0}^2 \int_{y=0}^2 (x\mathbf{u_x} + y\mathbf{u_y}) \bullet (\text{d}y\text{d}z(-\mathbf{u_y})) \\
		& = \int_{z=0}^2 \int_{x=0}^2 2\text{d}x\text{d}z + \int_{z=0}^2 \int_{y=0}^2 2\text{d}y\text{d}z \\
		& = \int_{z=0}^2 2x\rvert_{x=0}^2\text{d}z + \int_{z=0}^2 2y\rvert_{y=0}^2\text{d}z \\
		& = \int_{z=0}^2 4\text{d}z + \int_{z=0}^2 4\text{d}z \\
		& = 4z\rvert_{z=0}^2 + 4z\rvert_{z=0}^2 \\
		& = 8 + 8 \\
		& = 16
	\end{split}
\end{equation*}

\newpage

We can apply the divergence theorem to solve the above integral in a different way.

\begin{equation*}
	\begin{split}
		\oint \mathbf{A} \bullet \mathbf{ds} & = \int_{\Delta v} (\nabla \bullet \mathbf{A}) \text{d}v \\
		\int_{\Delta v} (\nabla \bullet \mathbf{A}) \text{d}v & = \int_{\Delta v} \left( \frac{\partial A_x}{\partial x} + \frac{\partial A_y}{\partial y} \right) \text{d}v \\
		& = \int_{\Delta v} (1 + 1)\text{d}v \\
		& = \int_{z=0}^2 \int_{y=0}^2 \int_{x=0}^2 2 \text{d}x \text{d}y \text{d}z \\
		& = \int_{z=0}^2 \int_{y=0}^2 2x\rvert_{x=0}^2 \text{d}y \text{d}z \\
		& = \int_{z=0}^2 \int_{y=0}^2 4 \text{d}y \text{d}z \\
		& = \int_{z=0}^2 4y\rvert_{y=0}^2 \text{d}z \\
		& = \int_{z=0}^2 8 \text{d}z \\
		& = 8z\rvert_{z=0}^2 \\
		& = 16
	\end{split}
\end{equation*}

\end{document}